{"cells":[{"cell_type":"markdown","id":"threatened-spotlight","metadata":{"id":"threatened-spotlight"},"source":["<h1 align=\"center\"> CSE 242 Lab Session, Fall 2022\n","\n","<h2 align=\"center\">Lab Session 1 (Sep 27th) --Swati & Fatemeh\n","\n"]},{"cell_type":"markdown","metadata":{"id":"uCyXZsQ7jLkc"},"source":["\n","**Task 1:** **Expectation** and **Variance** (a quick review)"],"id":"uCyXZsQ7jLkc"},{"cell_type":"markdown","metadata":{"id":"qCD5kquSjLkc"},"source":["**(1) Linear property of Expectation:** denote $X$ as the random variable, for any constants $a, b\\in \\mathbb{R}$, the expectation of $Y=aX+b$ is:\n","$$\\mathbf{E}[aX+b]=a\\mathbf{E}[X]+b$$\n","\n","**(2) Expectation of two random variables $X_1, X_2$:** \n","\n","$$\\mathbf{E}[X_1+X_2]=\\mathbf{E}[X_1]+\\mathbf{E}[X_2]$$\n","\n","If $X_1$ $ X_2$ and $ X_3$ have the same distribution (with the same mean $\\mathbf{E}(X_1)$ and variance $\\text{Var}(X_1$), we can further have:\n","\n","$$\\mathbf{E}[X_1+X_2+X_3]=\\mathbf{E}[X_1]+\\mathbf{E}[X_2]+\\mathbf{E}[X_3]=3\\cdot \\mathbf{E}[X_1]$$\n","\n","\n","**(3) Definition of Variance:** the variance of a random variable $X$ is the expectation of the random variable $Y$, where $Y=(X-\\mathbf{E}[X])^2$:\n","\n","$$\\text{Var}(X)=\\mathbf{E}\\Big[(X-\\mathbf{E}[X])^2\\Big]$$\n","\n","**(4) The relationship between $\\text{Var}(X)$ and $\\mathbf{E}[X]$:** $$\\text{Var}(X)=\\mathbf{E}[X^2]-(\\mathbf{E}[X])^2$$\n","\n","**(5) Property 1 of Variance:** for any constants $a, b\\in \\mathbb{R}$,\n","\n","$$\\text{Var}(aX+b)=a^2\\text{Var}(X)$$\n","\n","Let $a=\\dfrac{1}{3}, b=0, X=X_1+X_2+X_3$, you will have:\n","\n","$$\\text{Var}(aX+b)=\\text{Var}\\Big(\\dfrac{X_1+X_2+X_3}{3}\\Big)=(\\dfrac{1}{3})^2\\text{Var}(X)=(\\dfrac{1}{3})^2\\text{Var}(X_1+X_2+X_3)$$\n","\n","**(6) Variance of two random variables $X_1, X_2$:** $$\\text{Var}[X_1+X_2]=\\text{Var}[X_1]+2\\cdot \\text{Cov}[X_1, X_2]+\\text{Var}[X_2]$$\n","\n","Typically, if $X_1$ and $X_2$ are independent, \n","\n","$$\\text{Cov}[X_1, X_2]=\\mathbf{E}[X_1X_2]-\\mathbf{E}[X_1]\\mathbf{E}[X_2]=0$$\n","\n","And we have: $\\text{Var}[X_1+X_2]=\\text{Var}[X_1]+\\text{Var}[X_2]$.\n","\n","\n","If $X_1$ and $ X_2$ have the same distribution (with the same mean $\\mathbf{E}(X_1)$ and variance $\\text{Var}(X_1$), we can further have:  $$\\text{Var}[X_1+X_2]=2\\cdot \\text{Var}[X_1]$$\n","\n","**(7) Variance of three random variables $X_1, X_2, X_3$:**\n","\n"," $$\\text{Var}[X_1+X_2+X_3]= \\text{Var}[X_1]+\\text{Var}[X_2]+\\text{Var}[X_3]+\\text{Cov}[X_1, X_2]+\\text{Cov}[X_1, X_3]+\\text{Cov}[X_2, X_3]$$\n","\n","----------------------------------\n","\n","(**Optional:**) the proof of $\\text{Var}[X_1]+2\\cdot \\text{Cov}[X_1, X_2]+\\text{Var}[X_2]$, which helps you figure out why the covariance term $\\text{Cov}$ appears.\n","\n","According to (4),\n","\n","$$\\text{Var}[X_1+X_2]=\\mathbf{E}\\Big[\\Big(X_1+X_2-\\mathbf{E}[X_1+X_2]\\Big)^2\\Big]$$\n","\n","$$=\\mathbf{E}\\Big[\\Big((X_1-\\mathbf{E}[X_1]) + (X_2-\\mathbf{E}[X_2])\\Big)^2\\Big]$$\n","\n","$$=\\mathbf{E}\\Big[(X_1-\\mathbf{E}[X_1])^2 + 2\\cdot (X_1-\\mathbf{E}[X_1])(X_2-\\mathbf{E}[X_2]) + (X_2-\\mathbf{E}[X_2])^2\\Big]$$\n","\n","$$=\\mathbf{E}\\Big[(X_1-\\mathbf{E}[X_1])^2\\Big] + 2\\cdot \\mathbf{E}\\Big[(X_1-\\mathbf{E}[X_1])(X_2-\\mathbf{E}[X_2])\\Big] + \\mathbf{E}\\Big(X_2-\\mathbf{E}[X_2])^2\\Big]$$\n","\n","$$=\\mathbf{E}\\Big[(X_1-\\mathbf{E}[X_1])^2\\Big] + 2\\cdot \\mathbf{E}\\Big[X_1X_2-X_2\\mathbf{E}[X_1]-X_1\\mathbf{E}[X_2]+\\mathbf{E}[X_1]\\mathbf{E}[X_2]\\Big] + \\mathbf{E}\\Big(X_2-\\mathbf{E}[X_2])^2\\Big]$$\n","\n","$$=\\mathbf{E}\\Big[(X_1-\\mathbf{E}[X_1])^2\\Big] + 2\\cdot\\underbrace{\\Big(\\mathbf{E}[X_1X_2]-\\mathbf{E}[X_1]\\mathbf{E}[X_2]\\Big)}_{\\text{defined as }\\text{Cov}[X_1, X_2]} + \\mathbf{E}\\Big(X_2-\\mathbf{E}[X_2])^2\\Big]$$\n","\n","$$=\\text{Var}[X_1]+2\\cdot \\text{Cov}[X_1, X_2]+\\text{Var}[X_2]$$\n"],"id":"qCD5kquSjLkc"},{"cell_type":"markdown","source":["**Task 2**. Review how to derive $E(X)$ and $\\text{Var$(X)$}$ for a sample distribution: \n","\n","\n","**Poisson Distribution**\n","\n","A discrete random variable X is said to have a Poisson distribution, with parameter ${\\displaystyle \\lambda >0}$, if it has a probability mass function given by\n","$$ {f_X}(x) = \\dfrac{\\lambda^x e^{-\\lambda}}{x!}$$\n","\n","\n","**Derivation for E(X):**\n","\n","\n","The expected value of a discrete random variable is defined as \n","\n","$$E(X)= \\sum_{x \\in X} x.{f_X}(x)$$\n","\n","With the probability mass function of the Poisson distribution, we will have:\n","\n","\\begin{align}\n","E(X) &= \\sum_{x=0}^{\\infty} x.\\dfrac{\\lambda^x e^{-\\lambda}}{x!} \\\\\n","&= \\sum_{x=1}^{\\infty} x.\\dfrac{\\lambda^x e^{-\\lambda}}{x!} \\\\\n","&= e^{-\\lambda}.\\sum_{x=1}^{\\infty} x.\\dfrac{\\lambda^x}{x!} \\\\\n","&= \\lambda e^{-\\lambda}.\\sum_{x=1}^{\\infty} \\dfrac{\\lambda^{x-1}}{(x-1)!}\n","\\end{align}\n","\n","Substituting $z=x-1$, we have $x= z+1$, and we get:\n","\n","$$ E(X) = \\lambda e^{-\\lambda}.\\sum_{z=0}^{\\infty} \\dfrac{\\lambda^{z}}{z!} $$\n","\n","using the power series expansion of the exponential function:\n","\n","$$e^x = \\sum_{n=0}^{\\infty}\\dfrac{x^n}{n!} $$\n","\n","\n","We will have:\n","\n","\\begin{align}\n","E(X) &= \\lambda e^{-\\lambda}.\\sum_{z=0}^{\\infty} \\dfrac{\\lambda^{z}}{z!} \\\\\n","&= \\lambda e^{-\\lambda}.e^\\lambda \\\\\n","&= \\lambda\n","\\end{align}\n","\n","**Derivation for Var(X):**\n","\n","$$ \\text{Var(X)}= E[X^2]-({E}[X])^2$$\n","\n","We know that:\n","\\begin{align}\n","E(X^2)&= \\sum_{x \\in X} x^2.{f_X}(x) \\\\\n","&= \\sum_{x=0}^{\\infty} x^2.\\dfrac{\\lambda^x e^{-\\lambda}}{x!} \\\\\n","&= \\lambda e^{-\\lambda} \\sum_{x=1}^{\\infty} x.\\dfrac{\\lambda^{x-1}}{(x-1)!} \\\\\n","&= \\lambda e^{-\\lambda}\\left(\\sum_{x=1}^{\\infty} (x-1).\\dfrac{\\lambda^{x-1}}{(x-1)!} + \\sum_{x=1}^{\\infty} \\dfrac{\\lambda^{x-1}}{(x-1)!}\\right) \\\\\n","&= \\lambda e^{-\\lambda}\\left(\\lambda\\sum_{x=2}^{\\infty} \\dfrac{\\lambda^{x-2}}{(x-2)!} + \\sum_{x=1}^{\\infty} \\dfrac{\\lambda^{x-1}}{(x-1)!}\\right)\n","\\end{align}\n","\n","Substituting $i= x-2$ and $j=x-1$, we will have:\n","\\begin{align}\n","E(X^2)&= \\lambda e^{-\\lambda}\\left(\\lambda\\sum_{i=0}^{\\infty}\\dfrac{\\lambda^{i}}{i!}+ \\sum_{j=0}^{\\infty}\\dfrac{\\lambda^{j}}{j!} \\right)\\\\\n","&= \\lambda e^{-\\lambda}(\\lambda e^\\lambda +e^\\lambda) \\\\\n","&= \\lambda^2 +\\lambda\n","\\end{align}\n","\n","Therefore:\n","\\begin{align}\n","\\text{Var(X)}&= E[X^2]-({E}[X])^2 \\\\\n","&= \\lambda^2 +\\lambda- \\lambda^2 \\\\\n","&= \\lambda\n","\\end{align}"],"metadata":{"id":"nuO21C89U2t9"},"id":"nuO21C89U2t9"},{"cell_type":"code","source":[],"metadata":{"id":"mZE7wsgvgB8P"},"id":"mZE7wsgvgB8P","execution_count":null,"outputs":[]}],"metadata":{"kernelspec":{"display_name":"Python 3","language":"python","name":"python3"},"language_info":{"codemirror_mode":{"name":"ipython","version":3},"file_extension":".py","mimetype":"text/x-python","name":"python","nbconvert_exporter":"python","pygments_lexer":"ipython3","version":"3.9.1-final"},"colab":{"provenance":[],"collapsed_sections":[]}},"nbformat":4,"nbformat_minor":5}